per/per_props_nat2.v
@@ -26,6 +26,7 @@
 
 
 Require Export natk.
+Require Export per_respects.
 Require Export per_props_nat.
 
 
@@ -339,16 +340,6 @@ Proof.
   - apply tequality_unit.
 Qed.
 
-(* !!MOVE *)
-Hint Resolve alphaeqc_trans : slow.
-Hint Resolve alphaeqc_sym : slow.
-
-Lemma respects_alphaeqc_alphaeqc {o} : respects2 alphaeqc (@alphaeqc o).
-Proof.
-  unfold respects2; dands; introv aeq1 aeq2; eauto 3 with slow.
-Qed.
-Hint Resolve respects_alphaeqc_alphaeqc : respects.
-
 Lemma lsubstc_mk_nat2nat {o} :
   forall w (s : @CSub o) c,
     alphaeqc (lsubstc mk_nat2nat w s c) nat2nat.
@@ -374,48 +365,6 @@ Proof.
   apply type_mkc_fun; dands; eauto 3 with slow.
 Qed.
 Hint Resolve type_nat2nat : slow.
-
-Lemma member_respects_alphaeqc_l {o} :
-  forall lib (t1 t2 T : @CTerm o),
-    alphaeqc t1 t2 -> member lib t1 T -> member lib t2 T.
-Proof.
-  introv aeq mem.
-  allunfold @member.
-  eapply equality_respects_alphaeqc_left;[exact aeq|].
-  eapply equality_respects_alphaeqc_right;[exact aeq|].
-  auto.
-Qed.
-
-Lemma member_respects_alphaeqc_r {o} :
-  forall lib (t T1 T2 : @CTerm o),
-    alphaeqc T1 T2 -> member lib t T1 -> member lib t T2.
-Proof.
-  introv aeq mem.
-  allunfold @member.
-  eapply alphaeqc_preserving_equality; eauto.
-Qed.
-
-Lemma respects_alphaeqc_member {o} :
-  forall (lib : @library o), respects2 alphaeqc (member lib).
-Proof.
-  introv; unfold respects2; dands; introv aeq1 aeq2; eauto 3 with slow.
-  - eapply member_respects_alphaeqc_l; eauto.
-  - eapply member_respects_alphaeqc_r; eauto.
-Qed.
-Hint Resolve respects_alphaeqc_member : respects.
-
-Lemma respects_alphaeqc_equorsq3 {o} :
-  forall lib (t1 t2 T1 T2 : @CTerm o),
-    alphaeqc T1 T2
-    -> equorsq lib t1 t2 T1
-    -> equorsq lib t1 t2 T2.
-Proof.
-  introv aeq e.
-  eauto 3 with slow.
-  pose proof (respects_alphaeqc_equorsq lib) as h.
-  destruct h as [h1 h]; repnd.
-  eapply h; eauto.
-Qed.
 
 Lemma equality_natk_to_tnat {o} :
   forall lib (n1 n2 k : @CTerm o),
