per/per_respects.v
@@ -1,0 +1,96 @@
+(*
+
+  Copyright 2014 Cornell University
+  Copyright 2015 Cornell University
+
+  This file is part of VPrl (the Verified Nuprl project).
+
+  VPrl is free software: you can redistribute it and/or modify
+  it under the terms of the GNU General Public License as published by
+  the Free Software Foundation, either version 3 of the License, or
+  (at your option) any later version.
+
+  VPrl is distributed in the hope that it will be useful,
+  but WITHOUT ANY WARRANTY; without even the implied warranty of
+  MERCHANTABILITY or FITNESS FOR A PARTICULAR PURPOSE.  See the
+  GNU General Public License for more details.
+
+  You should have received a copy of the GNU General Public License
+  along with VPrl.  Ifnot, see <http://www.gnu.org/licenses/>.
+
+
+  Website: http://nuprl.org/html/verification/
+  Authors: Abhishek Anand & Vincent Rahli
+
+*)
+
+Require Export per_props.
+
+
+(* !!MOVE *)
+Hint Resolve alphaeqc_trans : slow.
+Hint Resolve alphaeqc_sym : slow.
+
+Lemma respects_alphaeqc_alphaeqc {o} : respects2 alphaeqc (@alphaeqc o).
+Proof.
+  unfold respects2; dands; introv aeq1 aeq2; eauto 3 with slow.
+Qed.
+Hint Resolve respects_alphaeqc_alphaeqc : respects.
+
+Lemma member_respects_alphaeqc_l {o} :
+  forall lib (t1 t2 T : @CTerm o),
+    alphaeqc t1 t2 -> member lib t1 T -> member lib t2 T.
+Proof.
+  introv aeq mem.
+  allunfold @member.
+  eapply equality_respects_alphaeqc_left;[exact aeq|].
+  eapply equality_respects_alphaeqc_right;[exact aeq|].
+  auto.
+Qed.
+
+Lemma member_respects_alphaeqc_r {o} :
+  forall lib (t T1 T2 : @CTerm o),
+    alphaeqc T1 T2 -> member lib t T1 -> member lib t T2.
+Proof.
+  introv aeq mem.
+  allunfold @member.
+  eapply alphaeqc_preserving_equality; eauto.
+Qed.
+
+Lemma respects_alphaeqc_member {o} :
+  forall (lib : @library o), respects2 alphaeqc (member lib).
+Proof.
+  introv; unfold respects2; dands; introv aeq1 aeq2; eauto 3 with slow.
+  - eapply member_respects_alphaeqc_l; eauto.
+  - eapply member_respects_alphaeqc_r; eauto.
+Qed.
+Hint Resolve respects_alphaeqc_member : respects.
+
+Lemma respects_alphaeqc_equorsq3 {o} :
+  forall lib (t1 t2 T1 T2 : @CTerm o),
+    alphaeqc T1 T2
+    -> equorsq lib t1 t2 T1
+    -> equorsq lib t1 t2 T2.
+Proof.
+  introv aeq e.
+  eauto 3 with slow.
+  pose proof (respects_alphaeqc_equorsq lib) as h.
+  destruct h as [h1 h]; repnd.
+  eapply h; eauto.
+Qed.
+
+Lemma respects_alphaeqc_cequivc {p} : forall lib, respects2 alphaeqc (@cequivc p lib).
+Proof.
+  introv; unfolds_base; dands; introv Hr Heq; allsimpl;
+  try (complete (left; eauto 3 with nequality)).
+  - apply (cequivc_trans lib a' a b); auto; apply cequivc_sym; apply alphaeqc_implies_cequivc; auto.
+  - apply (cequivc_trans lib a b b'); auto; apply alphaeqc_implies_cequivc; auto.
+Qed.
+Hint Resolve respects_alphaeqc_cequivc : respects.
+
+
+(*
+*** Local Variables:
+*** coq-load-path: ("." "../util/" "../terms/" "../computation/" "../cequiv/" "../close/")
+*** End:
+*)
